cava/cava/Cava/Types.v
@@ -14,7 +14,7 @@
 (* limitations under the License.                                           *)
 (****************************************************************************)
 
-(* Require Import Program.Basics. *)
+Require Import Program.Basics.
 From Coq Require Import Ascii String.
 From Coq Require Import ZArith.
 From Coq Require Import Lists.List.
@@ -27,6 +27,8 @@ Import ListNotations.
 Import MonadNotation.
 Open Scope list_scope.
 Open Scope monad_scope.
+
+From Cava Require Import Signal.
 
 (******************************************************************************)
 (* shape describes the types of wires going into or out of a Cava circuit,    *)
@@ -126,14 +128,14 @@ Fixpoint bitsInPortShape (s : bundle) : nat :=
   | Tuple2 t1 t2 => bitsInPortShape t1 + bitsInPortShape t2
   end.
 
-(* The duplicated i and l parametere are a temporary work-around to allow
+(* The duplicated i and l pamrameters are a temporary work-around to allow
    well-founded recursion to be recognized.
    TODO(satnam): Rewrite with an appropriate well-foundedness proof.
 *)
-Fixpoint numberBitVec (offset : N) (i : list nat) (l : list nat) : @denoteBitVecWith nat N l :=
-  match l, i return @denoteBitVecWith nat N l with
-  | [], _         => 0%N
-  | [x], [_]      => map N.of_nat (seq (N.to_nat offset) x)
+Fixpoint numberBitVec (offset : N) (i : list nat) (l : list nat) : @denoteBitVecWith nat Signal l :=
+  match l, i return @denoteBitVecWith nat Signal l with
+  | [], _         => Wire 0%N
+  | [x], [_]      => map (compose Wire N.of_nat) (seq (N.to_nat offset) x)
   | x::xs, p::ps  => let z := N.of_nat (fold_left (fun x y => x * y) xs 1) in
                      map (fun w => numberBitVec (offset+w*z) ps xs) (map N.of_nat (seq 0 x))
   | _, _          => []
@@ -182,12 +184,12 @@ Fixpoint signalTy (T : Type) (s : shape) : Type :=
   | Tuple2 s1 s2  => prod (signalTy T s1) (signalTy T s2)
   end.
 
-Fixpoint numberPort (i : N) (inputs: bundle) : signalTy N inputs :=
-  match inputs return signalTy N inputs with
+Fixpoint numberPort (i : N) (inputs: bundle) : signalTy Signal inputs :=
+  match inputs return signalTy Signal inputs with
   | Empty => tt
   | One typ =>
-      match typ return denoteKindWith typ N with
-      | Bit => i
+      match typ return denoteKindWith typ Signal with
+      | Bit => Wire i
       | BitVec xs => numberBitVec i xs xs
       end
   | Tuple2 t1 t2 => let t1Size := bitsInPortShape t1 in
